.

src/program_proof/session/definitions.v
@@ -94,54 +94,39 @@ End Client.
 
 Section heap.
 
-  Definition operation_val (op:Slice.t*u64) : val :=
+  Definition operation_val (op: Slice.t*u64) : val :=
     (slice_val op.1, (#op.2, #()))%V.
 
   Theorem operation_val_t op : val_ty (operation_val op) (struct.t Operation).
-  Proof.
-    repeat constructor; auto.
-  Qed.
+  Proof. repeat constructor; auto. Qed.
 
   Hint Resolve operation_val_t : core.
 
   Global Instance operation_into_val : IntoVal (Slice.t*u64).
   Proof.
-    refine {| into_val.to_val := operation_val;
-             from_val := λ v, match v with
-                              | (slice_v, (#(LitInt d), #()))%V =>
-                                  match from_val slice_v with
-                                  | Some s => Some (s, d)
-                                  | None => None
-                                  end
-                              | _ => None
-                              end;
-             IntoVal_def := (IntoVal_def Slice.t, W64 0);
-           |}.
-    destruct v as [[a []] d]; done. 
+    refine (
+      {|
+        into_val.to_val := operation_val;
+        from_val v :=
+          match v with
+          | (slice_v, (#(LitInt d), #()))%V =>
+            match from_val slice_v with
+            | Some s => Some (s, d)
+            | None => None
+            end
+          | _ => None
+          end;
+        IntoVal_def := (IntoVal_def Slice.t, W64 0);
+      |}
+    ).
+    intros [[? ?] ?]; auto.
   Defined.
 
   #[global] Instance operation_into_val_for_type : IntoValForType (Slice.t*u64) (struct.t Operation).
   Proof. constructor; auto. Qed.
 
-  Definition message_val (msg:u64*u64*u64*u64*u64*Slice.t*u64*u64*Slice.t*u64*u64*u64*u64*u64*u64*Slice.t*u64*u64) : val :=
-    (#msg.1.1.1.1.1.1.1.1.1.1.1.1.1.1.1.1.1,
-       (#msg.1.1.1.1.1.1.1.1.1.1.1.1.1.1.1.1.2,
-          (#msg.1.1.1.1.1.1.1.1.1.1.1.1.1.1.1.2,
-             (#msg.1.1.1.1.1.1.1.1.1.1.1.1.1.1.2,
-                (#msg.1.1.1.1.1.1.1.1.1.1.1.1.1.2,
-                   (slice_val msg.1.1.1.1.1.1.1.1.1.1.1.1.2,
-                      (#msg.1.1.1.1.1.1.1.1.1.1.1.2,
-                         (#msg.1.1.1.1.1.1.1.1.1.1.2,
-                            (slice_val msg.1.1.1.1.1.1.1.1.1.2,
-                               (#msg.1.1.1.1.1.1.1.1.2,
-                                  (#msg.1.1.1.1.1.1.1.2,
-                                     (#msg.1.1.1.1.1.1.2,
-                                        (#msg.1.1.1.1.1.2,
-                                           (#msg.1.1.1.1.2,
-                                              (#msg.1.1.1.2,
-                                                 (slice_val msg.1.1.2,
-                                                    (#msg.1.2,
-                                                       (#msg.2, #()))))))))))))))))))%V.
+  Definition message_val (msg: u64*u64*u64*u64*u64*Slice.t*u64*u64*Slice.t*u64*u64*u64*u64*u64*u64*Slice.t*u64*u64) : val :=
+    (#msg.1.1.1.1.1.1.1.1.1.1.1.1.1.1.1.1.1, (#msg.1.1.1.1.1.1.1.1.1.1.1.1.1.1.1.1.2, (#msg.1.1.1.1.1.1.1.1.1.1.1.1.1.1.1.2, (#msg.1.1.1.1.1.1.1.1.1.1.1.1.1.1.2, (#msg.1.1.1.1.1.1.1.1.1.1.1.1.1.2, (slice_val msg.1.1.1.1.1.1.1.1.1.1.1.1.2, (#msg.1.1.1.1.1.1.1.1.1.1.1.2, (#msg.1.1.1.1.1.1.1.1.1.1.2, (slice_val msg.1.1.1.1.1.1.1.1.1.2, (#msg.1.1.1.1.1.1.1.1.2, (#msg.1.1.1.1.1.1.1.2, (#msg.1.1.1.1.1.1.2, (#msg.1.1.1.1.1.2, (#msg.1.1.1.1.2, (#msg.1.1.1.2, (slice_val msg.1.1.2, (#msg.1.2, (#msg.2, #()))))))))))))))))))%V.
 
   Lemma redefine_message_val
     : message_val = @SessionPrelude.value_of (tuple_of [u64,u64,u64,u64,u64,Slice.t,u64,u64,Slice.t,u64,u64,u64,u64,u64,u64,Slice.t,u64,u64]) _.
@@ -150,85 +135,37 @@ Section heap.
   Defined.
 
   Theorem message_val_t msg : val_ty (message_val msg) (struct.t server.Message).
-  Proof.
-    repeat constructor; auto.
-  Qed.
+  Proof. repeat constructor; auto. Qed.
 
   Hint Resolve message_val_t : core.
 
-  Definition message_from_val (v : val) : option (u64*u64*u64*u64*u64*Slice.t*u64*u64*Slice.t*u64*u64*u64*u64*u64*u64*Slice.t*u64*u64) :=
+  Definition message_from_val (v: val) : option (u64*u64*u64*u64*u64*Slice.t*u64*u64*Slice.t*u64*u64*u64*u64*u64*u64*Slice.t*u64*u64) :=
     match v with
-    | (#(LitInt MessageType),
-         (#(LitInt C2S_Client_Id),
-            (#(LitInt C2S_Server_Id),
-               (#(LitInt C2S_Client_OperationType),
-                  (#(LitInt C2S_Client_Data),
-                     (C2S_Client_VersionVector,
-                        (#(LitInt S2S_Gossip_Sending_ServerId),
-                           (#(LitInt S2S_Gossip_Receiving_ServerId),
-                              (S2S_Gossip_Operations,
-                                 (#(LitInt S2S_Gossip_Index),
-                                    (#(LitInt S2S_Acknowledge_Gossip_Sending_ServerId),
-                                       (#(LitInt S2S_Acknowledge_Gossip_Receiving_ServerId),
-                                          (#(LitInt S2S_Acknowledge_Gossip_Index),
-                                             (#(LitInt S2C_Client_OperationType),
-                                                (#(LitInt S2C_Client_Data),
-                                                   (S2C_Client_VersionVector,
-                                                      (#(LitInt S2C_Server_Id),
-                                                         (#(LitInt S2C_Client_Number), #()))))))))))))))))))%V =>
-        match ((from_val C2S_Client_VersionVector: option Slice.t),
-                 (from_val S2S_Gossip_Operations: option Slice.t),
-                   (from_val S2C_Client_VersionVector: option Slice.t)) with
-        | (Some s1, Some s2, Some s3) => Some (MessageType,
-                                                 C2S_Client_Id,
-                                                   C2S_Server_Id,
-                                                     C2S_Client_OperationType,
-                                                       C2S_Client_Data,
-                                                         s1, 
-                                                           S2S_Gossip_Sending_ServerId,
-                                                             S2S_Gossip_Receiving_ServerId, s2, S2S_Gossip_Index,
-                                                               S2S_Acknowledge_Gossip_Sending_ServerId,
-                                                                 S2S_Acknowledge_Gossip_Receiving_ServerId,
-                                                                   S2S_Acknowledge_Gossip_Index,
-                                                                     S2C_Client_OperationType,
-                                                                       S2C_Client_Data,
-                                                                         s3,
-                                                                           S2C_Server_Id,
-                                                                             S2C_Client_Number)
-        | _ => None
-        end
+    | (#(LitInt MessageType), (#(LitInt C2S_Client_Id), (#(LitInt C2S_Server_Id), (#(LitInt C2S_Client_OperationType), (#(LitInt C2S_Client_Data), (C2S_Client_VersionVector, (#(LitInt S2S_Gossip_Sending_ServerId), (#(LitInt S2S_Gossip_Receiving_ServerId), (S2S_Gossip_Operations, (#(LitInt S2S_Gossip_Index), (#(LitInt S2S_Acknowledge_Gossip_Sending_ServerId), (#(LitInt S2S_Acknowledge_Gossip_Receiving_ServerId), (#(LitInt S2S_Acknowledge_Gossip_Index), (#(LitInt S2C_Client_OperationType), (#(LitInt S2C_Client_Data), (S2C_Client_VersionVector, (#(LitInt S2C_Server_Id), (#(LitInt S2C_Client_Number), #()))))))))))))))))))%V =>
+      match (slice_IntoVal.(from_val) C2S_Client_VersionVector, slice_IntoVal.(from_val) S2S_Gossip_Operations, slice_IntoVal.(from_val) S2C_Client_VersionVector) with
+      | (Some s1, Some s2, Some s3) => Some (MessageType, C2S_Client_Id, C2S_Server_Id, C2S_Client_OperationType, C2S_Client_Data, s1, S2S_Gossip_Sending_ServerId, S2S_Gossip_Receiving_ServerId, s2, S2S_Gossip_Index, S2S_Acknowledge_Gossip_Sending_ServerId, S2S_Acknowledge_Gossip_Receiving_ServerId, S2S_Acknowledge_Gossip_Index, S2C_Client_OperationType, S2C_Client_Data, s3, S2C_Server_Id, S2C_Client_Number)
+      | _ => None
+      end
     | _ => None
     end.
-  
-  Global Instance message_into_val : IntoVal (u64*u64*u64*u64*u64*Slice.t*u64*u64*Slice.t*u64*u64*u64*u64*u64*u64*Slice.t*u64*u64).
+
+  #[global] Instance message_into_val : IntoVal (u64*u64*u64*u64*u64*Slice.t*u64*u64*Slice.t*u64*u64*u64*u64*u64*u64*Slice.t*u64*u64).
   Proof.
-    refine {| into_val.to_val := message_val;
-             from_val := message_from_val ;
-             IntoVal_def := (W64 0, W64 0, W64 0, W64 0, W64 0,
-                               IntoVal_def Slice.t, W64 0, W64 0,
-                                 IntoVal_def Slice.t,
-                                   W64 0, W64 0, W64 0, W64 0, W64 0,
-                                     W64 0, IntoVal_def Slice.t,
-                                       W64 0, W64 0);
-           |}.
-    destruct v. repeat destruct p. simpl. f_equal.
-    destruct t1. destruct t0. destruct t.
-    simpl. auto.
-  Defined. 
+    refine (
+      {|
+        into_val.to_val := message_val;
+        from_val := message_from_val;
+        IntoVal_def := (W64 0, W64 0, W64 0, W64 0, W64 0, IntoVal_def Slice.t, W64 0, W64 0, IntoVal_def Slice.t, W64 0, W64 0, W64 0, W64 0, W64 0, W64 0, IntoVal_def Slice.t, W64 0, W64 0);
+      |}
+    ).
+    do 17 destruct v as [v ?]; simpl; repeat lazymatch goal with [ t : Slice.t |- _ ] => destruct t end; auto.
+  Defined.
 
   #[global] Instance message_into_val_for_type : IntoValForType (u64*u64*u64*u64*u64*Slice.t*u64*u64*Slice.t*u64*u64*u64*u64*u64*u64*Slice.t*u64*u64) (struct.t server.Message).
   Proof. constructor; auto. simpl. repeat split; auto. Qed.
 
   Definition server_val (s: u64*u64*Slice.t*Slice.t*Slice.t*Slice.t*Slice.t*Slice.t) : val :=
-    (#s.1.1.1.1.1.1.1,
-       (#s.1.1.1.1.1.1.2,
-          (slice_val s.1.1.1.1.1.2,
-             (slice_val s.1.1.1.1.2,
-                (slice_val s.1.1.1.2,
-                   (slice_val s.1.1.2,
-                      (slice_val s.1.2,
-                         (slice_val s.2,
-                            #()))))))))%V.
+    (#s.1.1.1.1.1.1.1, (#s.1.1.1.1.1.1.2, (slice_val s.1.1.1.1.1.2, (slice_val s.1.1.1.1.2, (slice_val s.1.1.1.2, (slice_val s.1.1.2, (slice_val s.1.2, (slice_val s.2, #()))))))))%V.
 
   Lemma redefine_server_val
     : server_val = @SessionPrelude.value_of (tuple_of [u64,u64,Slice.t,Slice.t,Slice.t,Slice.t,Slice.t,Slice.t]) _.
@@ -237,64 +174,37 @@ Section heap.
   Defined.
 
   Theorem server_val_t server : val_ty (server_val server) (struct.t Server).
-  Proof.
-    repeat constructor; auto.
-  Qed.
+  Proof. repeat constructor; auto. Qed.
 
   Hint Resolve server_val_t : core.
 
-  Definition server_from_val (v : val) : option (u64*u64*Slice.t*Slice.t*Slice.t*Slice.t*Slice.t*Slice.t) :=
+  Definition server_from_val (v: val) : option (u64*u64*Slice.t*Slice.t*Slice.t*Slice.t*Slice.t*Slice.t) :=
     match v with
-    | (#(LitInt Id),
-         (#(LitInt NumberOfServers),
-            (UnsatisfiedRequests,
-               (VectorClock,
-                  (OperationsPerformed,
-                     (MyOperations,
-                        (PendingOperations,
-                           (GossipAcknowledgements, #()))))))))%V =>
-        match ((from_val UnsatisfiedRequests: option Slice.t),
-                 (from_val VectorClock: option Slice.t),
-                   (from_val OperationsPerformed: option Slice.t),
-                     (from_val MyOperations: option Slice.t),
-                       (from_val PendingOperations: option Slice.t),
-                         (from_val GossipAcknowledgements: option Slice.t)
-              ) with
-        | (Some s1, Some s2, Some s3, Some s4, Some s5, Some s6) =>
-            Some (Id, NumberOfServers, s1, s2, s3, s4, s5, s6)
-        | _ => None
-        end
+    | (#(LitInt Id), (#(LitInt NumberOfServers), (UnsatisfiedRequests, (VectorClock, (OperationsPerformed, (MyOperations, (PendingOperations, (GossipAcknowledgements, #()))))))))%V =>
+      match (slice_IntoVal.(from_val) UnsatisfiedRequests, slice_IntoVal.(from_val) VectorClock, slice_IntoVal.(from_val) OperationsPerformed, slice_IntoVal.(from_val) MyOperations, slice_IntoVal.(from_val) PendingOperations, slice_IntoVal.(from_val) GossipAcknowledgements) with
+      | (Some s1, Some s2, Some s3, Some s4, Some s5, Some s6) => Some (Id, NumberOfServers, s1, s2, s3, s4, s5, s6)
+      | _ => None
+      end
     | _ => None
     end.
   
-  Global Instance server_into_val : IntoVal (u64*u64*Slice.t*Slice.t*Slice.t*Slice.t*Slice.t*Slice.t).
+  #[global] Instance server_into_val : IntoVal (u64*u64*Slice.t*Slice.t*Slice.t*Slice.t*Slice.t*Slice.t).
   Proof.
-    refine {| into_val.to_val := server_val;
-             from_val := server_from_val ;
-             IntoVal_def := (W64 0, W64 0, 
-                               IntoVal_def Slice.t,
-                                 IntoVal_def Slice.t,
-                                   IntoVal_def Slice.t,
-                                     IntoVal_def Slice.t,
-                                       IntoVal_def Slice.t,
-                                         IntoVal_def Slice.t);
-           |}.
-    destruct v. repeat destruct p. simpl. f_equal.
-    destruct t0. destruct t. destruct t1. destruct t2. destruct t3.
-    destruct t4. 
-    simpl. auto.
+    refine (
+      {|
+        into_val.to_val := server_val;
+        from_val := server_from_val ;
+        IntoVal_def := (W64 0, W64 0, IntoVal_def Slice.t, IntoVal_def Slice.t, IntoVal_def Slice.t, IntoVal_def Slice.t, IntoVal_def Slice.t, IntoVal_def Slice.t);
+      |}
+    ).
+    do 7 destruct v as [v ?]; simpl; repeat lazymatch goal with [ t : Slice.t |- _ ] => destruct t end; auto.
   Defined.
 
   #[global] Instance server_into_val_for_type : IntoValForType (u64*u64*Slice.t*Slice.t*Slice.t*Slice.t*Slice.t*Slice.t) (struct.t server.Server).
   Proof. constructor; auto. simpl. repeat split; auto. Qed.
 
   Definition client_val (c:u64*u64*Slice.t*Slice.t*u64) : val :=
-    (#c.1.1.1.1,
-       (#c.1.1.1.2,
-          (slice_val c.1.1.2,
-             (slice_val c.1.2 ,
-                (#c.2 ,
-                   #())))))%V.
+    (#c.1.1.1.1, (#c.1.1.1.2, (slice_val c.1.1.2, (slice_val c.1.2, (#c.2, #())))))%V.
 
   Lemma redefine_client_val
     : client_val = @SessionPrelude.value_of (tuple_of [u64,u64,Slice.t,Slice.t,u64]) _.
@@ -309,36 +219,26 @@ Section heap.
 
   Hint Resolve client_val_t : core.
 
-  Definition client_from_val (v : val) : option (u64*u64*Slice.t*Slice.t*u64) :=
+  Definition client_from_val (v: val) : option (u64*u64*Slice.t*Slice.t*u64) :=
     match v with
-    | (#(LitInt Id),
-         (#(LitInt NumberOfServers),
-            (WriteVersionVector,
-               (ReadVersionVector,
-                  (#(LitInt SessionSemantic),
-                     #())))))%V =>
-        match ((from_val WriteVersionVector: option Slice.t),
-                 (from_val ReadVersionVector: option Slice.t))
-        with
-        | (Some s1, Some s2) =>
-            Some (Id, NumberOfServers, s1, s2, SessionSemantic)
-        | _ => None
-        end
+    | (#(LitInt Id), (#(LitInt NumberOfServers), (WriteVersionVector, (ReadVersionVector, (#(LitInt SessionSemantic), #())))))%V =>
+      match (slice_IntoVal.(from_val) WriteVersionVector, slice_IntoVal.(from_val) ReadVersionVector) with
+      | (Some s1, Some s2) => Some (Id, NumberOfServers, s1, s2, SessionSemantic)
+      | _ => None
+      end
     | _ => None
     end.
-  
-  Global Instance client_into_val : IntoVal (u64*u64*Slice.t*Slice.t*u64).
+
+  #[global] Instance client_into_val : IntoVal (u64*u64*Slice.t*Slice.t*u64).
   Proof.
-    refine {| into_val.to_val := client_val;
-             from_val := client_from_val ;
-             IntoVal_def := (W64 0, W64 0, 
-                               IntoVal_def Slice.t,
-                                 IntoVal_def Slice.t,
-                                   W64 0);
-           |}.
-    destruct v. repeat destruct p. simpl. f_equal.
-    destruct t0. destruct t.
-    simpl. auto.
+    refine (
+      {|
+        into_val.to_val := client_val;
+        from_val := client_from_val ;
+        IntoVal_def := (W64 0, W64 0, IntoVal_def Slice.t, IntoVal_def Slice.t, W64 0);
+      |}
+    ).
+    do 5 destruct v as [v ?]; simpl; repeat lazymatch goal with [ t : Slice.t |- _ ] => destruct t end; auto.
   Defined.
 
   #[global] Instance client_into_val_for_type : IntoValForType (u64*u64*Slice.t*Slice.t*u64) (struct.t client.Client).
@@ -347,7 +247,7 @@ Section heap.
   Context `{hG: !heapGS Σ}.
 
   Definition is_operation (opv: Slice.t*u64) (op: Operation.t) (len_opv: nat) : iProp Σ :=
-    (* Data *) ⌜opv.2 = op.(Operation.Data) /\ u64_ge_CONSTANT op.(Operation.Data)⌝ ∗
+    ⌜opv.2 = op.(Operation.Data)⌝ ∗
     ⌜len_opv = length op.(Operation.VersionVector) /\ Forall u64_ge_CONSTANT op.(Operation.VersionVector)⌝ ∗
     own_slice_small opv.1 uint64T DfracDiscarded op.(Operation.VersionVector).
 
@@ -359,7 +259,7 @@ Section heap.
     ⌜msgv!(1) = msg.(Message.C2S_Client_Id) /\ u64_ge_CONSTANT msg.(Message.C2S_Client_Id)⌝ ∗
     ⌜msgv!(2) = msg.(Message.C2S_Server_Id) /\ u64_ge_CONSTANT msg.(Message.C2S_Server_Id)⌝ ∗
     ⌜msgv!(3) = msg.(Message.C2S_Client_OperationType) /\ u64_ge_CONSTANT msg.(Message.C2S_Client_OperationType)⌝ ∗
-    (* Data *) ⌜msgv!(4) = msg.(Message.C2S_Client_Data) /\ u64_ge_CONSTANT msg.(Message.C2S_Client_Data)⌝ ∗
+    ⌜msgv!(4) = msg.(Message.C2S_Client_Data)⌝ ∗
     own_slice_small msgv!(5) uint64T (DfracOwn 1) msg.(Message.C2S_Client_VersionVector) ∗
     ⌜len_c2s = length msg.(Message.C2S_Client_VersionVector) /\ Forall u64_ge_CONSTANT msg.(Message.C2S_Client_VersionVector)⌝ ∗
     ⌜msgv!(6) = msg.(Message.S2S_Gossip_Sending_ServerId) /\ u64_ge_CONSTANT msg.(Message.S2S_Gossip_Sending_ServerId)⌝ ∗
@@ -370,7 +270,7 @@ Section heap.
     ⌜msgv!(11) = msg.(Message.S2S_Acknowledge_Gossip_Receiving_ServerId) /\ u64_ge_CONSTANT msg.(Message.S2S_Acknowledge_Gossip_Receiving_ServerId)⌝ ∗
     ⌜msgv!(12) = msg.(Message.S2S_Acknowledge_Gossip_Index) /\ u64_ge_CONSTANT msg.(Message.S2S_Acknowledge_Gossip_Index)⌝ ∗
     ⌜msgv!(13) = msg.(Message.S2C_Client_OperationType) /\ u64_ge_CONSTANT msg.(Message.S2C_Client_OperationType)⌝ ∗
-    (* Data *) ⌜msgv!(14) = msg.(Message.S2C_Client_Data) /\ u64_ge_CONSTANT msg.(Message.S2C_Client_Data)⌝ ∗
+    ⌜msgv!(14) = msg.(Message.S2C_Client_Data)⌝ ∗
     own_slice_small msgv!(15) uint64T (DfracOwn 1) msg.(Message.S2C_Client_VersionVector) ∗
     ⌜len_s2c = length msg.(Message.S2C_Client_VersionVector) /\ Forall u64_ge_CONSTANT msg.(Message.S2C_Client_VersionVector)⌝ ∗
     ⌜msgv!(16) = msg.(Message.S2C_Server_Id) /\ u64_ge_CONSTANT msg.(Message.S2C_Server_Id)⌝ ∗
